cleanup version for the finite type of regt.

noc/setup.v
@@ -66,119 +66,28 @@ Module Instances.
   Derive Signature for reg_t.
   Derive NoConfusion for reg_t.
   
-  Equations fin_idx {n} (r: (reg_t (S n))) : nat :=
-    fin_idx (router _ (@F1 n')   state) := 2 * n';
-    fin_idx (router _ (@FS n' _) state) := 2 * n';
-    fin_idx (router _ (@F1 n')   downstream) := 2 * n' + 1;
-    fin_idx (router _ (@FS n' _) downstream) := 2 * n' + 1.
-
-  (* TODO move rename to [widen_le_t] *)
-  Equations widen_fin_left {m} (H: m <<= S (S m)) : S m <<= S (S m) :=
-    widen_fin_left (m:=m') H' := le_S _ _ (le_n (S m')).
-
-  Equations widen_fin_left0 {m} (H: 0 <<= S (S m)) : S 0 <<= S (S m) :=
-    widen_fin_left0 (m:=0)    H' := widen_fin_left H';
-    widen_fin_left0 (m:=S m') (le_S _ _ H') := le_S _ _ (widen_fin_left0 H').
-
-  Equations widen_le_t_S {n m} (H: n <<= m) : S n <<= S m :=
-    widen_le_t_S (n:=n') (m:=?(n')) (le_n ?(n')) :=  le_n (S n');
-    widen_le_t_S (n:=n') (m:=?(S m'))  (le_S n' m' H') :=
-     le_S _ _ (widen_le_t_S H').
-
-  Equations fin_elems' n m (H: n <<= m) : list (reg_t (S m)) :=
-    fin_elems' 0      0     _               := cons (router 0 F1 state) (cons (router 0 F1 downstream) nil);
-    fin_elems' 0     (S 0) (le_S 0 ?(0) H') :=
-      let f1 := FS (@F1 0) in
-      cons (router (S 0) f1 state) (cons (router (S 0) f1 downstream) nil);
-
-  fin_elems' 0     (S (S m')) H' :=
-    let f1 := FS (widen_fin (widen_fin_left0 H') (@F1 0)) in
-    cons (router (S (S m')) f1 state) (cons (router (S (S m')) f1 downstream) nil);
-
-  fin_elems' (S n') (S m') H' with fin_elems' n' (S m') (le_t_inj H') :=
-    | tl := let f1 := widen_fin (widen_le_t_S H') (@F1 (S n')) in
-            cons (router (S m') f1 state)
-              (cons (router (S m') f1 downstream) tl).   
-
-  Definition fin_elems {n} : list (reg_t (S n)) :=
-    fin_elems' n n (le_n n).
-
-  Equations lift {m} (l: list (reg_t m)) : list (reg_t (S m)) :=
-    lift nil := nil;
-    lift (cons (router m f s) tl) with lift tl => {
-        | tl' := cons (router (S m) (FS f) s) tl'
-      }.
-
   Equations lift_router {m} (r: reg_t m) : reg_t (S m) :=
     lift_router (router m f s) := router (S m) (FS f) s.
   
-  Equations fin_elems'' {m} : list (reg_t (S m)) :=
-    fin_elems'' (m:=0)      := cons (router 0 F1 state) (cons (router 0 F1 downstream) nil);
-    fin_elems'' (m:=(S m')) with fin_elems'' => {
+  Equations regt_elems {m} : list (reg_t (S m)) :=
+    regt_elems (m:=0)      := cons (router 0 F1 state) (cons (router 0 F1 downstream) nil);
+    regt_elems (m:=(S m')) with regt_elems => {
       | tl := cons (router (S m') (@F1 (S m')) state)
                 (cons (router (S m') (@F1 (S m')) downstream)
                    (map lift_router tl))
         }.
 
-  Equations fin_idx'' {n} (idx:nat) (r: (reg_t (S n))) : nat :=
-    fin_idx'' idx' (router 0 (FS f) r)      := absurd_fin f;
-    fin_idx'' idx' (router (S m) (FS f) r)  := fin_idx'' (S idx') (router m f r);
-    fin_idx'' idx' (router m F1 state)      := 2 * idx' + 1;
-    fin_idx'' idx' (router m F1 downstream) := 2 * idx'.
-
-  Definition fin_idx' {n} (r: (reg_t (S n))) : nat := fin_idx'' 0 r.
-
-  Fixpoint finite_index_Fint {n} (f : Fin.t n) : nat :=
-    match f with
-    | Fin.F1 => 0
-    | Fin.FS f' => S (finite_index_Fint f')
-    end.
-
-  Definition a := @F1 2.
-  Definition b := FS a.
-
-  Check a.
-  Check b.
-  Compute (finite_index_Fint a).
-  Compute (finite_index_Fint b).
-
-  Compute (fin_idx' (router 2 a state)).
-  Compute (fin_idx' (router 2 a downstream)).
-  Compute (fin_idx' (router 3 b state)).
-  Compute (fin_idx' (router 3 b downstream)).
-
-  Definition c := FS (FS (FS (@F1 1))).
-
-  Compute (finite_index_Fint c).
-
-  Fixpoint finite_elements_Fint {n} : list (Fin.t n) :=
-    match n with
-    | O => []
-    | S _ => Fin.F1 :: map Fin.FS finite_elements_Fint
-    end.
-
-  Definition mod5 : list (Fin.t 5) := finite_elements_Fint.
-
-  Compute mod5.
-  Compute c.
-  Compute (finite_index_Fint c).
-
-  Definition router_mod5 := router 4 c state.
-  Definition routers_mod5 : list (reg_t 5) := fin_elems''.
-
-  Compute routers_mod5.
-
-  Equations fint_idx {n} (r: (reg_t (S n))) : nat :=
-    fint_idx (router 0 (FS f) r)              := absurd_fin f;
-    fint_idx (router m F1 state)      := 0;
-    fint_idx (router m F1 downstream) := 1;
-    fint_idx (router (S m) (FS f) r) := S (S (fint_idx (router m f r))).
+  Equations regt_idx {n} (r: (reg_t (S n))) : nat :=
+    regt_idx (router 0 (FS f) r)      := absurd_fin f;
+    regt_idx (router m F1 state)      := 0;
+    regt_idx (router m F1 downstream) := 1;
+    regt_idx (router (S m) (FS f) r)  := S (S (regt_idx (router m f r))).
 
   Lemma regt_error {n} :
     forall (r: (reg_t (S n))),
-      List.nth_error fin_elems'' (fint_idx r) = Some r.
+      List.nth_error regt_elems (regt_idx r) = Some r.
   Proof.
-    induction n; intros r; depelim r; depelim t; destruct r; simp fint_idx; simp fin_elems''; simpl; try (reflexivity || depelim t).
+    induction n; intros r; depelim r; depelim t; destruct r; simp regt_idx; simp regt_elems; simpl; try (reflexivity || depelim t).
     - specialize (IHn (router n F1 state)).
       fold (lift_router (router n F1 state)).
       apply map_nth_error.
@@ -198,22 +107,22 @@ Module Instances.
   Qed.
 
   Lemma regt_injective {n} :
-    NoDup (List.map (@fint_idx n) fin_elems'').
+    NoDup (List.map (@regt_idx n) regt_elems).
   Proof.
-    assert (is_seq : (List.map (@fint_idx n) fin_elems'') = seq 0 ((S n)*2)).
-    induction n; simp fin_elems''; simp fint_idx; try reflexivity.
+    assert (is_seq : (List.map (@regt_idx n) regt_elems) = seq 0 ((S n)*2)).
+    induction n; simp regt_elems; simp regt_idx; try reflexivity.
     - do 2 rewrite map_cons.
       rewrite map_map.
       erewrite map_ext.
       2:{
         intros a.
-        depelim a; simp lift_router; simp fint_idx.
-        instantiate (1:= fun x => S (S (fint_idx x))).
+        depelim a; simp lift_router; simp regt_idx.
+        instantiate (1:= fun x => S (S (regt_idx x))).
         cbn beta.
         exact eq_refl.
       }
       rewrite <- map_map.
-      rewrite <- (map_map _ S fin_elems'').
+      rewrite <- (map_map _ S regt_elems).
       rewrite IHn.
       cbn.
       repeat f_equal.
@@ -222,13 +131,11 @@ Module Instances.
     - rewrite is_seq. apply seq_NoDup.
   Qed.
 
-  About Build_FiniteType.
-
   Instance Fin_regt {n} : FiniteType (reg_t (S n)) :=
     Build_FiniteType
       (reg_t (S n))
-      fint_idx
-      fin_elems''
+      regt_idx
+      regt_elems
       regt_error
       regt_injective.
 
